Update to latest Comparse (`bl*` -> `tls_*`)

fstar/MLS.NetworkTypes.fst
@@ -2,9 +2,9 @@ module MLS.NetworkTypes
 
 open Comparse
 
-type hpke_public_key_nt (bytes:Type0) {|bytes_like bytes|} = blbytes bytes ({min=1; max=(pow2 16)-1})
+type hpke_public_key_nt (bytes:Type0) {|bytes_like bytes|} = tls_bytes bytes ({min=1; max=(pow2 16)-1})
 val ps_hpke_public_key_nt: #bytes:Type0 -> {|bytes_like bytes|} -> parser_serializer bytes (hpke_public_key_nt bytes)
-let ps_hpke_public_key_nt #bytes #bl = ps_blbytes _
+let ps_hpke_public_key_nt #bytes #bl = ps_tls_bytes _
 
 //This is from draft 12+
 (*
@@ -14,9 +14,9 @@ let ps_key_package_ref_nt #bytes #bl = ps_lbytes 16
 *)
 
 //This is from draft 12
-type key_package_ref_nt (bytes:Type0) {|bytes_like bytes|} = blbytes bytes ({min=0; max=255})
+type key_package_ref_nt (bytes:Type0) {|bytes_like bytes|} = tls_bytes bytes ({min=0; max=255})
 val ps_key_package_ref_nt: #bytes:Type0 -> {|bytes_like bytes|} -> parser_serializer bytes (key_package_ref_nt bytes)
-let ps_key_package_ref_nt #bytes #bl = ps_blbytes _
+let ps_key_package_ref_nt #bytes #bl = ps_tls_bytes _
 
 type proposal_ref_nt (bytes:Type0) {|bytes_like bytes|} = lbytes bytes 16
 val ps_proposal_ref_nt: #bytes:Type0 -> {|bytes_like bytes|} -> parser_serializer bytes (proposal_ref_nt bytes)
@@ -24,15 +24,15 @@ let ps_proposal_ref_nt #bytes #bl = ps_lbytes 16
 
 
 noeq type hpke_ciphertext_nt (bytes:Type0) {|bytes_like bytes|} = {
-  kem_output: blbytes bytes ({min=0; max=(pow2 16)-1});
-  ciphertext: blbytes bytes ({min=0; max=(pow2 16)-1});
+  kem_output: tls_bytes bytes ({min=0; max=(pow2 16)-1});
+  ciphertext: tls_bytes bytes ({min=0; max=(pow2 16)-1});
 }
 
 %splice [ps_hpke_ciphertext_nt] (gen_parser (`hpke_ciphertext_nt))
 
 noeq type update_path_node_nt (bytes:Type0) {|bytes_like bytes|} = {
   public_key: hpke_public_key_nt bytes;
-  encrypted_path_secret: blseq bytes ps_hpke_ciphertext_nt ({min=0; max=(pow2 32)-1});
+  encrypted_path_secret: tls_seq bytes ps_hpke_ciphertext_nt ({min=0; max=(pow2 32)-1});
 }
 
 %splice [ps_update_path_node_nt] (gen_parser (`update_path_node_nt))
@@ -63,21 +63,21 @@ type signature_scheme_nt =
 %splice [ps_signature_scheme_nt] (gen_parser (`signature_scheme_nt))
 
 noeq type basic_credential_nt (bytes:Type0) {|bytes_like bytes|} = {
-  identity: blbytes bytes ({min=0; max=(pow2 16)-1});
+  identity: tls_bytes bytes ({min=0; max=(pow2 16)-1});
   signature_scheme: signature_scheme_nt;
-  signature_key: blbytes bytes ({min=0; max=(pow2 16)-1});
+  signature_key: tls_bytes bytes ({min=0; max=(pow2 16)-1});
 }
 
 %splice [ps_basic_credential_nt] (gen_parser (`basic_credential_nt))
 
-type certificate_nt (bytes:Type0) {|bytes_like bytes|} = blbytes bytes ({min=0; max=(pow2 16)-1})
+type certificate_nt (bytes:Type0) {|bytes_like bytes|} = tls_bytes bytes ({min=0; max=(pow2 16)-1})
 
 val ps_certificate_nt: #bytes:Type0 -> {|bytes_like bytes|} -> parser_serializer bytes (certificate_nt bytes)
-let ps_certificate_nt #bytes #bl = ps_blbytes _
+let ps_certificate_nt #bytes #bl = ps_tls_bytes _
 
 noeq type credential_nt (bytes:Type0) {|bytes_like bytes|} =
   | C_basic: [@@@ with_num_tag 2 1] basic_credential_nt bytes -> credential_nt bytes
-  | C_x509: [@@@ with_num_tag 2 2] blseq bytes ps_certificate_nt ({min=1; max=(pow2 32)-1}) -> credential_nt bytes
+  | C_x509: [@@@ with_num_tag 2 2] tls_seq bytes ps_certificate_nt ({min=1; max=(pow2 32)-1}) -> credential_nt bytes
 
 %splice [ps_credential_nt] (gen_parser (`credential_nt))
 
@@ -93,7 +93,7 @@ type extension_type_nt: eqtype =
 
 noeq type extension_nt (bytes:Type0) {|bytes_like bytes|} = {
   extension_type: extension_type_nt;
-  extension_data: blbytes bytes ({min=0; max=(pow2 32)-1});
+  extension_data: tls_bytes bytes ({min=0; max=(pow2 32)-1});
 }
 
 %splice [ps_extension_nt] (gen_parser (`extension_nt))
@@ -102,9 +102,9 @@ noeq type key_package_tbs_nt (bytes:Type0) {|bytes_like bytes|} = {
   version: protocol_version_nt;
   cipher_suite: cipher_suite_nt;
   public_key: hpke_public_key_nt bytes;
-  endpoint_id: blbytes bytes ({min=0; max=255});
+  endpoint_id: tls_bytes bytes ({min=0; max=255});
   credential: credential_nt bytes;
-  extensions: blseq bytes ps_extension_nt ({min=8; max=(pow2 32)-1});
+  extensions: tls_seq bytes ps_extension_nt ({min=8; max=(pow2 32)-1});
 }
 
 %splice [ps_key_package_tbs_nt] (gen_parser (`key_package_tbs_nt))
@@ -113,7 +113,7 @@ instance parseable_serializeable_key_package_tbs_nt (bytes:Type0) {|bytes_like b
 
 noeq type key_package_nt (bytes:Type0) {|bytes_like bytes|} = {
   tbs: key_package_tbs_nt bytes;
-  signature: blbytes bytes ({min=0; max=(pow2 16)-1});
+  signature: tls_bytes bytes ({min=0; max=(pow2 16)-1});
 }
 
 %splice [ps_key_package_nt] (gen_parser (`key_package_nt))
@@ -122,25 +122,25 @@ instance parseable_serializeable_key_package_nt (bytes:Type0) {|bytes_like bytes
 
 noeq type update_path_nt (bytes:Type0) {|bytes_like bytes|} = {
   leaf_key_package: key_package_nt bytes;
-  nodes: blseq bytes ps_update_path_node_nt ({min=0; max=(pow2 32)-1});
+  nodes: tls_seq bytes ps_update_path_node_nt ({min=0; max=(pow2 32)-1});
 }
 
 %splice [ps_update_path_nt] (gen_parser (`update_path_nt))
 
 noeq type group_context_nt (bytes:Type0) {|bytes_like bytes|} = {
-  group_id: blbytes bytes ({min=0; max=255});
+  group_id: tls_bytes bytes ({min=0; max=255});
   epoch: nat_lbytes 8;
-  tree_hash: blbytes bytes ({min=0; max=255});
-  confirmed_transcript_hash: blbytes bytes ({min=0; max=255});
-  extensions: blseq bytes ps_extension_nt ({min=0; max=(pow2 32)-1});
+  tree_hash: tls_bytes bytes ({min=0; max=255});
+  confirmed_transcript_hash: tls_bytes bytes ({min=0; max=255});
+  extensions: tls_seq bytes ps_extension_nt ({min=0; max=(pow2 32)-1});
 }
 
 %splice [ps_group_context_nt] (gen_parser (`group_context_nt))
 
 noeq type parent_node_nt (bytes:Type0) {|bytes_like bytes|} = {
   public_key: hpke_public_key_nt bytes;
-  parent_hash: blbytes bytes ({min=0; max=255});
-  unmerged_leaves: blseq bytes (ps_nat_lbytes #bytes 4) ({min=0; max=(pow2 32)-1});
+  parent_hash: tls_bytes bytes ({min=0; max=255});
+  unmerged_leaves: tls_seq bytes (ps_nat_lbytes #bytes 4) ({min=0; max=(pow2 32)-1});
 }
 
 %splice [ps_parent_node_nt] (gen_parser (`parent_node_nt))
@@ -175,10 +175,10 @@ let ps_option #bytes #bl #a ps_a =
     | Some x -> (|1, x|)
   )
 
-type ratchet_tree_nt (bytes:Type0) {|bytes_like bytes|} = blseq bytes (ps_option ps_node_nt) ({min=1; max=(pow2 32)-1})
+type ratchet_tree_nt (bytes:Type0) {|bytes_like bytes|} = tls_seq bytes (ps_option ps_node_nt) ({min=1; max=(pow2 32)-1})
 
 val ps_ratchet_tree_nt: #bytes:Type0 -> {|bytes_like bytes|} -> parser_serializer bytes (ratchet_tree_nt bytes)
-let ps_ratchet_tree_nt #bytes #bl = ps_blseq (ps_option ps_node_nt) _
+let ps_ratchet_tree_nt #bytes #bl = ps_tls_seq (ps_option ps_node_nt) _
 
 type psk_type_nt =
   | PSKT_external: [@@@ with_num_tag 1 1] unit -> psk_type_nt
@@ -188,15 +188,15 @@ type psk_type_nt =
 %splice [ps_psk_type_nt] (gen_parser (`psk_type_nt))
 
 noeq type pre_shared_key_id_nt (bytes:Type0) {|bytes_like bytes|} =
-  //| PSKI_reserved: [@@@ with_tag (PSKT_reserved ())] psk_nonce:blbytes bytes ({min=0; max=255}) -> pre_shared_key_id_nt bytes
-  | PSKI_external: [@@@ with_tag (PSKT_external ())] psk_id:blbytes bytes ({min=0; max=255}) -> psk_nonce:blbytes bytes ({min=0; max=255}) -> pre_shared_key_id_nt bytes
-  | PSKI_reinit: [@@@ with_tag (PSKT_reinit ())] psk_group_id:blbytes bytes ({min=0; max=255}) -> psk_epoch:nat_lbytes 8 -> psk_nonce:blbytes bytes ({min=0; max=255}) -> pre_shared_key_id_nt bytes
-  | PSKI_branch: [@@@ with_tag (PSKT_branch ())] psk_group_id:blbytes bytes ({min=0; max=255}) -> psk_epoch:nat_lbytes 8 -> psk_nonce:blbytes bytes ({min=0; max=255}) -> pre_shared_key_id_nt bytes
+  //| PSKI_reserved: [@@@ with_tag (PSKT_reserved ())] psk_nonce:tls_bytes bytes ({min=0; max=255}) -> pre_shared_key_id_nt bytes
+  | PSKI_external: [@@@ with_tag (PSKT_external ())] psk_id:tls_bytes bytes ({min=0; max=255}) -> psk_nonce:tls_bytes bytes ({min=0; max=255}) -> pre_shared_key_id_nt bytes
+  | PSKI_reinit: [@@@ with_tag (PSKT_reinit ())] psk_group_id:tls_bytes bytes ({min=0; max=255}) -> psk_epoch:nat_lbytes 8 -> psk_nonce:tls_bytes bytes ({min=0; max=255}) -> pre_shared_key_id_nt bytes
+  | PSKI_branch: [@@@ with_tag (PSKT_branch ())] psk_group_id:tls_bytes bytes ({min=0; max=255}) -> psk_epoch:nat_lbytes 8 -> psk_nonce:tls_bytes bytes ({min=0; max=255}) -> pre_shared_key_id_nt bytes
 
 %splice [ps_pre_shared_key_id_nt] (gen_parser (`pre_shared_key_id_nt))
 
 noeq type pre_shared_keys_nt (bytes:Type0) {|bytes_like bytes|} = {
-  psks: blseq bytes ps_pre_shared_key_id_nt ({min=0; max=(pow2 16)-1});
+  psks: tls_seq bytes ps_pre_shared_key_id_nt ({min=0; max=(pow2 16)-1});
 }
 
 %splice [ps_pre_shared_keys_nt] (gen_parser (`pre_shared_keys_nt))
@@ -238,16 +238,16 @@ noeq type pre_shared_key_nt (bytes:Type0) {|bytes_like bytes|} = {
 %splice [ps_pre_shared_key_nt] (gen_parser (`pre_shared_key_nt))
 
 noeq type reinit_nt (bytes:Type0) {|bytes_like bytes|} = {
-  group_id: blbytes bytes ({min=0; max=255});
+  group_id: tls_bytes bytes ({min=0; max=255});
   version: protocol_version_nt;
   cipher_suite: cipher_suite_nt;
-  extensions: blseq bytes ps_extension_nt ({min=0; max=(pow2 32)-1})
+  extensions: tls_seq bytes ps_extension_nt ({min=0; max=(pow2 32)-1})
 }
 
 %splice [ps_reinit_nt] (gen_parser (`reinit_nt))
 
 noeq type external_init_nt (bytes:Type0) {|bytes_like bytes|} = {
-  kem_output: blbytes bytes ({min=0; max=(pow2 16)-1})
+  kem_output: tls_bytes bytes ({min=0; max=(pow2 16)-1})
 }
 
 %splice [ps_external_init_nt] (gen_parser (`external_init_nt))
@@ -261,13 +261,13 @@ noeq type message_range_nt (bytes:Type0) {|bytes_like bytes|} = {
 %splice [ps_message_range_nt] (gen_parser (`message_range_nt))
 
 noeq type app_ack_nt (bytes:Type0) {|bytes_like bytes|} = {
-  received_ranges: blseq bytes ps_message_range_nt ({min=0; max=(pow2 32)-1})
+  received_ranges: tls_seq bytes ps_message_range_nt ({min=0; max=(pow2 32)-1})
 }
 
 %splice [ps_app_ack_nt] (gen_parser (`app_ack_nt))
 
 noeq type group_context_extensions_nt (bytes:Type0) {|bytes_like bytes|} = {
-  extensions: blseq bytes ps_extension_nt ({min=0; max=(pow2 32)-1});
+  extensions: tls_seq bytes ps_extension_nt ({min=0; max=(pow2 32)-1});
 }
 
 %splice [ps_group_context_extensions_nt] (gen_parser (`group_context_extensions_nt))
@@ -293,7 +293,7 @@ noeq type proposal_or_ref_nt (bytes:Type0) {|bytes_like bytes|} =
 %splice [ps_proposal_or_ref_nt] (gen_parser (`proposal_or_ref_nt))
 
 noeq type commit_nt (bytes:Type0) {|bytes_like bytes|} = {
-  proposals: blseq bytes ps_proposal_or_ref_nt ({min=0; max=(pow2 32)-1});
+  proposals: tls_seq bytes ps_proposal_or_ref_nt ({min=0; max=(pow2 32)-1});
   [@@@ with_parser #bytes (ps_option ps_update_path_nt)]
   path: option (update_path_nt bytes);
 }
@@ -309,7 +309,7 @@ type sender_type_nt =
 
 noeq type sender_nt (bytes:Type0) {|bytes_like bytes|} =
   | S_member: [@@@ with_tag (ST_member ())] member:key_package_ref_nt bytes -> sender_nt bytes
-  | S_preconfigured: [@@@ with_tag (ST_preconfigured ())] external_key_id:blbytes bytes ({min=0; max=255}) -> sender_nt bytes
+  | S_preconfigured: [@@@ with_tag (ST_preconfigured ())] external_key_id:tls_bytes bytes ({min=0; max=255}) -> sender_nt bytes
   | S_new_member: [@@@ with_tag (ST_new_member ())] unit -> sender_nt bytes
 
 %splice [ps_sender_nt] (gen_parser (`sender_nt))
@@ -321,7 +321,7 @@ type wire_format_nt =
 %splice [ps_wire_format_nt] (gen_parser (`wire_format_nt))
 
 noeq type mac_nt (bytes:Type0) {|bytes_like bytes|} = {
-  mac_value: blbytes bytes ({min=0; max=255});
+  mac_value: tls_bytes bytes ({min=0; max=255});
 }
 
 %splice [ps_mac_nt] (gen_parser (`mac_nt))
@@ -334,19 +334,19 @@ type content_type_nt =
 %splice [ps_content_type_nt] (gen_parser (`content_type_nt))
 
 noeq type mls_content_nt (bytes:Type0) {|bytes_like bytes|} =
-  | MC_application: [@@@ with_tag (CT_application ())] blbytes bytes ({min=0; max=(pow2 32)-1}) -> mls_content_nt bytes
+  | MC_application: [@@@ with_tag (CT_application ())] tls_bytes bytes ({min=0; max=(pow2 32)-1}) -> mls_content_nt bytes
   | MC_proposal: [@@@ with_tag (CT_proposal ())] proposal_nt bytes -> mls_content_nt bytes
   | MC_commit: [@@@ with_tag (CT_commit ())] commit_nt bytes -> mls_content_nt bytes
 
 %splice [ps_mls_content_nt] (gen_parser (`mls_content_nt))
 
 noeq type mls_plaintext_nt (bytes:Type0) {|bytes_like bytes|} = {
-  group_id: blbytes bytes ({min=0; max=255});
+  group_id: tls_bytes bytes ({min=0; max=255});
   epoch: nat_lbytes 8;
   sender: sender_nt bytes;
-  authenticated_data: blbytes bytes ({min=0; max=(pow2 32)-1});
+  authenticated_data: tls_bytes bytes ({min=0; max=(pow2 32)-1});
   content: mls_content_nt bytes;
-  signature: blbytes bytes ({min=0; max=(pow2 16)-1});
+  signature: tls_bytes bytes ({min=0; max=(pow2 16)-1});
   [@@@ with_parser #bytes (ps_option ps_mac_nt)]
   confirmation_tag: option (mac_nt bytes);
   [@@@ with_parser #bytes (ps_option ps_mac_nt)]
@@ -356,12 +356,12 @@ noeq type mls_plaintext_nt (bytes:Type0) {|bytes_like bytes|} = {
 %splice [ps_mls_plaintext_nt] (gen_parser (`mls_plaintext_nt))
 
 noeq type mls_ciphertext_nt (bytes:Type0) {|bytes_like bytes|} = {
-  group_id: blbytes bytes ({min=0; max=255});
+  group_id: tls_bytes bytes ({min=0; max=255});
   epoch: nat_lbytes 8;
   content_type: content_type_nt;
-  authenticated_data: blbytes bytes ({min=0; max=(pow2 32)-1});
-  encrypted_sender_data: blbytes bytes ({min=0; max=255});
-  ciphertext: blbytes bytes ({min=0; max=(pow2 32)-1});
+  authenticated_data: tls_bytes bytes ({min=0; max=(pow2 32)-1});
+  encrypted_sender_data: tls_bytes bytes ({min=0; max=255});
+  ciphertext: tls_bytes bytes ({min=0; max=(pow2 32)-1});
 }
 
 %splice [ps_mls_ciphertext_nt] (gen_parser (`mls_ciphertext_nt))
@@ -369,23 +369,23 @@ noeq type mls_ciphertext_nt (bytes:Type0) {|bytes_like bytes|} = {
 val mls_message_content_nt: bytes:Type0 -> {|bytes_like bytes|} -> content_type_nt -> Type0
 let mls_message_content_nt bytes #bl content_type =
   match content_type with
-  | CT_application () -> blbytes bytes ({min=0; max=(pow2 32)-1})
+  | CT_application () -> tls_bytes bytes ({min=0; max=(pow2 32)-1})
   | CT_proposal () -> proposal_nt bytes
   | CT_commit () -> commit_nt bytes
 
 val ps_mls_message_content_nt: #bytes:Type0 -> {|bytes_like bytes|} -> content_type:content_type_nt -> parser_serializer bytes (mls_message_content_nt bytes content_type)
 let ps_mls_message_content_nt #bytes #bl content_type =
   match content_type with
-  | CT_application () -> ps_blbytes ({min=0; max=(pow2 32)-1})
+  | CT_application () -> ps_tls_bytes ({min=0; max=(pow2 32)-1})
   | CT_proposal () -> ps_proposal_nt
   | CT_commit () -> ps_commit_nt
 
 noeq type mls_ciphertext_content_nt (bytes:Type0) {|bytes_like bytes|} (content_type: content_type_nt) = {
   content: mls_message_content_nt bytes content_type;
-  signature: blbytes bytes ({min=0; max=(pow2 16)-1});
+  signature: tls_bytes bytes ({min=0; max=(pow2 16)-1});
   [@@@ with_parser #bytes (ps_option ps_mac_nt)]
   confirmation_tag: option (mac_nt bytes);
-  padding: blbytes bytes ({min=0; max=(pow2 16)-1});
+  padding: tls_bytes bytes ({min=0; max=(pow2 16)-1});
 }
 
 %splice [ps_mls_ciphertext_content_nt] (gen_parser (`mls_ciphertext_content_nt))
@@ -393,10 +393,10 @@ noeq type mls_ciphertext_content_nt (bytes:Type0) {|bytes_like bytes|} (content_
 instance parseable_serializeable_mls_ciphertext_content_nt (bytes:Type0) {|bytes_like bytes|} (content_type:content_type_nt): parseable_serializeable bytes (mls_ciphertext_content_nt bytes content_type) = mk_parseable_serializeable (ps_mls_ciphertext_content_nt content_type)
 
 noeq type mls_ciphertext_content_aad_nt (bytes:Type0) {|bytes_like bytes|} = {
-  group_id: blbytes bytes ({min=0; max=255});
+  group_id: tls_bytes bytes ({min=0; max=255});
   epoch: nat_lbytes 8;
   content_type: content_type_nt;
-  authenticated_data: blbytes bytes ({min=0; max=(pow2 32)-1});
+  authenticated_data: tls_bytes bytes ({min=0; max=(pow2 32)-1});
 }
 
 %splice [ps_mls_ciphertext_content_aad_nt] (gen_parser (`mls_ciphertext_content_aad_nt))
@@ -414,7 +414,7 @@ noeq type mls_sender_data_nt (bytes:Type0) {|bytes_like bytes|} = {
 instance parseable_serializeable_mls_sender_data_nt (bytes:Type0) {|bytes_like bytes|}: parseable_serializeable bytes (mls_sender_data_nt bytes) = mk_parseable_serializeable ps_mls_sender_data_nt
 
 noeq type mls_sender_data_aad_nt (bytes:Type0) {|bytes_like bytes|} = {
-  group_id: blbytes bytes ({min=0; max=255});
+  group_id: tls_bytes bytes ({min=0; max=255});
   epoch: nat_lbytes 8;
   content_type: content_type_nt;
 }
@@ -426,12 +426,12 @@ instance parseable_serializeable_mls_sender_data_aad_nt (bytes:Type0) {|bytes_li
 //Structure used for confirmed transcript hash
 noeq type mls_plaintext_commit_content_nt (bytes:Type0) {|bytes_like bytes|} = {
   wire_format: wire_format_nt;
-  group_id: blbytes bytes ({min=0; max=255});
+  group_id: tls_bytes bytes ({min=0; max=255});
   epoch: nat_lbytes 8;
   sender: sender_nt bytes;
-  authenticated_data: blbytes bytes ({min=0; max=(pow2 32)-1});
+  authenticated_data: tls_bytes bytes ({min=0; max=(pow2 32)-1});
   content: mls_content_nt bytes; //is a commit
-  signature: blbytes bytes ({min=0; max=(pow2 16)-1});
+  signature: tls_bytes bytes ({min=0; max=(pow2 16)-1});
 }
 
 %splice [ps_mls_plaintext_commit_content_nt] (gen_parser (`mls_plaintext_commit_content_nt))
@@ -451,10 +451,10 @@ instance parseable_serializeable_mls_plaintext_commit_auth_data_nt (bytes:Type0)
 //Warning: you have to prepend the group context if sender.sender_type is ST_member!
 noeq type mls_plaintext_tbs_nt (bytes:Type0) {|bytes_like bytes|} = {
   wire_format: wire_format_nt;
-  group_id: blbytes bytes ({min=0; max=255});
+  group_id: tls_bytes bytes ({min=0; max=255});
   epoch: nat_lbytes 8;
   sender: sender_nt bytes;
-  authenticated_data: blbytes bytes ({min=0; max=(pow2 32)-1});
+  authenticated_data: tls_bytes bytes ({min=0; max=(pow2 32)-1});
   content: mls_content_nt bytes;
 }
 
@@ -465,7 +465,7 @@ instance parseable_serializeable_mls_plaintext_tbs_nt (bytes:Type0) {|bytes_like
 //Warning: you have to prepend the group context if tbs.sender.sender_type is ST_member!
 noeq type mls_plaintext_tbm_nt (bytes:Type0) {|bytes_like bytes|} = {
   tbs: mls_plaintext_tbs_nt bytes;
-  signature: blbytes bytes ({min=0; max=(pow2 16)-1});
+  signature: tls_bytes bytes ({min=0; max=(pow2 16)-1});
   [@@@ with_parser #bytes (ps_option ps_mac_nt)]
   confirmation_tag: option (mac_nt bytes);
 }
@@ -475,12 +475,12 @@ noeq type mls_plaintext_tbm_nt (bytes:Type0) {|bytes_like bytes|} = {
 instance parseable_serializeable_mls_plaintext_tbm_nt (bytes:Type0) {|bytes_like bytes|}: parseable_serializeable bytes (mls_plaintext_tbm_nt bytes) = mk_parseable_serializeable ps_mls_plaintext_tbm_nt
 
 noeq type group_info_tbs_nt (bytes:Type0) {|bytes_like bytes|} = {
-  group_id: blbytes bytes ({min=0; max=255});
+  group_id: tls_bytes bytes ({min=0; max=255});
   epoch: nat_lbytes 8;
-  tree_hash: blbytes bytes ({min=0; max=255});
-  confirmed_transcript_hash: blbytes bytes ({min=0; max=255});
-  group_context_extensions: blbytes bytes ({min=0; max=(pow2 32)-1});
-  other_extensions: blbytes bytes ({min=0; max=(pow2 32)-1});
+  tree_hash: tls_bytes bytes ({min=0; max=255});
+  confirmed_transcript_hash: tls_bytes bytes ({min=0; max=255});
+  group_context_extensions: tls_bytes bytes ({min=0; max=(pow2 32)-1});
+  other_extensions: tls_bytes bytes ({min=0; max=(pow2 32)-1});
   confirmation_tag: mac_nt bytes;
   signer: key_package_ref_nt bytes;
 }
@@ -491,7 +491,7 @@ instance parseable_serializeable_group_info_tbs_nt (bytes:Type0) {|bytes_like by
 
 noeq type group_info_nt (bytes:Type0) {|bytes_like bytes|} = {
   tbs: group_info_tbs_nt bytes;
-  signature: blbytes bytes ({min=0; max=(pow2 16)-1});
+  signature: tls_bytes bytes ({min=0; max=(pow2 16)-1});
 }
 
 %splice [ps_group_info_nt] (gen_parser (`group_info_nt))
@@ -500,13 +500,13 @@ noeq type group_info_nt (bytes:Type0) {|bytes_like bytes|} = {
 instance parseable_serializeable_group_info_nt (bytes:Type0) {|bytes_like bytes|}: parseable_serializeable bytes (group_info_nt bytes) = mk_parseable_serializeable ps_group_info_nt
 
 noeq type path_secret_nt (bytes:Type0) {|bytes_like bytes|} = {
-  path_secret: blbytes bytes ({min=0; max=255});
+  path_secret: tls_bytes bytes ({min=0; max=255});
 }
 
 %splice [ps_path_secret_nt] (gen_parser (`path_secret_nt))
 
 noeq type group_secrets_nt (bytes:Type0) {|bytes_like bytes|} = {
-  joiner_secret: blbytes bytes ({min=1; max=255});
+  joiner_secret: tls_bytes bytes ({min=1; max=255});
   [@@@ with_parser #bytes (ps_option ps_path_secret_nt)]
   path_secret: option (path_secret_nt bytes);
   psks: pre_shared_keys_nt bytes;
@@ -526,8 +526,8 @@ noeq type encrypted_group_secrets_nt (bytes:Type0) {|bytes_like bytes|} = {
 noeq type welcome_nt (bytes:Type0) {|bytes_like bytes|} = {
   version: protocol_version_nt;
   cipher_suite: cipher_suite_nt;
-  secrets: blseq bytes ps_encrypted_group_secrets_nt ({min=0; max=(pow2 32)-1});
-  encrypted_group_info: blbytes bytes ({min=1; max=(pow2 32)-1});
+  secrets: tls_seq bytes ps_encrypted_group_secrets_nt ({min=0; max=(pow2 32)-1});
+  encrypted_group_info: tls_bytes bytes ({min=1; max=(pow2 32)-1});
 }
 
 %splice [ps_welcome_nt] (gen_parser (`welcome_nt))
